LeanPy/Data/Type/Ref.lean
@@ -31,6 +31,14 @@ abbrev base? (self : TypeRef) : Option TypeRef :=
 abbrev name (self : TypeRef) : String :=
   self.data.name
 
+@[simp, inherit_doc PyType.isBaseType]
+abbrev isBaseType (self : TypeRef) : Bool :=
+  self.data.isBaseType
+
+@[simp, inherit_doc PyType.isBuiltin]
+abbrev isBuiltin (self : TypeRef) : Bool :=
+  self.data.isBuiltin
+
 @[simp, inherit_doc PyType.isTypeSubclass]
 abbrev isTypeSubclass (self : TypeRef) : Bool :=
   self.data.isTypeSubclass
@@ -46,116 +54,3 @@ abbrev isStrSubclass (self : TypeRef) : Bool :=
 @[simp, inherit_doc PyType.IsValidObject]
 abbrev IsValidObject (self : TypeRef) : ObjectProp.Raw :=
   self.data.IsValidObject
-
-/-- The type's method resolution order. -/
-@[inline] def mro (self : TypeRef) : List TypeRef :=
-  self :: go self.toRawTypeRef.data
-where go self :=
-  match self with
-  | {base? := none, ..} => []
-  | {base? := some base, ..} => ⟨base⟩ :: go base.data
-termination_by structural self
-
-@[inline] def baseMro (self : TypeRef) : List TypeRef :=
-  self.base?.elim [] mro
-
-theorem baseMro_eq_elim : baseMro self = self.base?.elim [] mro := rfl
-
-theorem mro_eq_cons_baseMro : mro self = self :: baseMro self := by
-  unfold mro mro.go
-  simp only [baseMro_eq_elim, Option.elim, Option.map, base?, data]
-  match self.toRawTypeRef.data with
-  | {base? := none, ..} => rfl
-  | {base? := some base, ..} => simp only [mro]
-
-instance : SizeOf TypeRef := ⟨(·.baseMro.length)⟩
-
-@[simp] theorem sizeOf_def {self : TypeRef} :
-  sizeOf self = self.baseMro.length
-:= rfl
-
-@[simp] theorem length_mro : (mro self).length = self.baseMro.length + 1 := by
-  simp [mro_eq_cons_baseMro]
-
-theorem mem_mro_iff : ty ∈ mro self ↔ ty = self ∨ ty ∈ baseMro self := by
-  simp [mro_eq_cons_baseMro]
-
-@[simp] theorem self_mem_mro : self ∈ mro self := by
-  simp [mro_eq_cons_baseMro]
-
-@[simp] theorem baseMro_subset_mro : baseMro self ⊆ mro self := by
-  simp [mro_eq_cons_baseMro]
-
-private theorem sup_mem_baseMro_sub :
-  sup ∈ baseMro sub → ∀ {ty}, ty ∈ baseMro sup → ty ∈ baseMro sub
-:= by
-  match h_sub:sub.base? with
-  | none =>
-    simp only [baseMro_eq_elim, h_sub, Option.elim_none, List.not_mem_nil]
-    intro sup_eq_sub
-    intro ty
-    simp [sup_eq_sub]
-  | some base =>
-    have sub_baseMro : sub.baseMro = mro base := by
-      simp [h_sub, baseMro_eq_elim]
-    simp only [sub_baseMro, mem_mro_iff]
-    intro h ty
-    intro ty_mem
-    apply Or.inr
-    cases h with
-    | inl sup_eq_sub => simpa [sup_eq_sub] using ty_mem
-    | inr sup_mem_mro_base => exact sup_mem_baseMro_sub sup_mem_mro_base ty_mem
-termination_by sub
-decreasing_by simp [sub_baseMro]
-
-private theorem sup_mem_mro_sub :
-  sup ∈ mro sub → ∀ {ty}, ty ∈ mro sup → ty ∈ mro sub
-:= by
-  simp only [mem_mro_iff]
-  rintro ⟨_ | _⟩ _ ⟨_ | _⟩
-  · simp
-  · simp [*]
-  · simp [*]
-  · apply Or.inr
-    next sup_mem ty ty_mem =>
-    exact sup_mem_baseMro_sub sup_mem ty_mem
-
-def Subtype (self other : TypeRef) : Prop :=
-  other ∈ self.mro
-
-instance : HasSubset TypeRef := ⟨TypeRef.Subtype⟩
-
-theorem subset_iff_mem_mro : a ⊆ b ↔ b ∈ mro a := Iff.rfl
-
-def SSubtype (self other : TypeRef) : Prop :=
-  other ∈ self.baseMro
-
-instance : HasSSubset TypeRef := ⟨TypeRef.SSubtype⟩
-
-theorem SSubtype.iff_mem_baseMro : a ⊂ b ↔ b ∈ baseMro a := Iff.rfl
-
-theorem Subtype.iff_eq_or_mem_baseMro : a ⊆ b ↔ (a = b ∨ b ∈ baseMro a) := by
-  grind [subset_iff_mem_mro, mem_mro_iff]
-
-theorem Subtype.iff_eq_or_ssubset {a b : TypeRef} : a ⊆ b ↔ (a = b ∨ a ⊂ b) := by
-  rw [Subtype.iff_eq_or_mem_baseMro, SSubtype.iff_mem_baseMro]
-
-@[simp] theorem Subtype.rfl {self : TypeRef} : self ⊆ self := self_mem_mro
-
-@[simp] theorem Subtype.refl (self : TypeRef) : self ⊆ self := self_mem_mro
-
-theorem SSubtype.trans {a b c : TypeRef} : a ⊂ b → b ⊂ c → a ⊂ c := by
-  simp only [SSubtype.iff_mem_baseMro]
-  exact fun h₁ h₂ => sup_mem_baseMro_sub h₁ h₂
-
-instance : Trans (SSubset : TypeRef → TypeRef → Prop) SSubset SSubset :=
-  ⟨SSubtype.trans⟩
-
-theorem Subtype.trans {a b c : TypeRef} : a ⊆ b → b ⊆ c → a ⊆ c  := by
-  simp only [subset_iff_mem_mro]
-  exact fun h₁ h₂ => sup_mem_mro_sub h₁ h₂
-
-instance : Trans (Subset : TypeRef → TypeRef → Prop) Subset Subset :=
-  ⟨Subtype.trans⟩
-
-end TypeRef
