LeanPy/Data/Type/Mro.lean
@@ -1,0 +1,136 @@
+/-
+Copyright (c) 2025 Mac Malone. All rights reserved.
+Released under the Apache 2.0 license as described in the file LICENSE.
+Authors: Mac Malone
+-/
+import LeanPy.Data.Type.Ref
+
+namespace LeanPy
+
+/-- The type's method resolution order (excluding itself). -/
+@[inline] def RawTypeRef.baseMro (self : RawTypeRef) : List TypeRef :=
+  go self.data
+where go self :=
+  match self with
+  | {base? := none, ..} => []
+  | {base? := some base, ..} => ⟨base⟩ :: go base.data
+termination_by structural self
+
+/-- The type's method resolution order (excluding itself). -/
+@[inline] def PyType.baseMro (self : PyType) : List TypeRef :=
+  self.base?.elim [] fun base => ⟨base⟩ :: RawTypeRef.baseMro base
+
+namespace TypeRef
+
+/-- The type's method resolution order. -/
+@[inline] def mro (self : TypeRef) : List TypeRef :=
+  self :: self.toRawTypeRef.baseMro
+
+/-- The type's method resolution order (excluding itself). -/
+@[inline] def baseMro (self : TypeRef) : List TypeRef :=
+  self.base?.elim [] mro
+
+theorem baseMro_eq_elim : baseMro self = self.base?.elim [] mro := rfl
+
+theorem baseMro_eq_data_baseMro : baseMro self = self.data.baseMro := by
+  simp only [baseMro_eq_elim, PyType.baseMro, base?]
+  cases self.data.base? <;> simp only [Option.elim, Option.map, mro]
+
+theorem mro_eq_cons_baseMro : mro self = self :: baseMro self := by
+  unfold mro RawTypeRef.baseMro RawTypeRef.baseMro.go
+  simp only [baseMro_eq_elim, Option.elim, Option.map, base?, data]
+  match self.toRawTypeRef.data with
+  | {base? := none, ..} => rfl
+  | {base? := some base, ..} => simp only [mro, RawTypeRef.baseMro]
+
+instance : SizeOf TypeRef := ⟨(·.baseMro.length)⟩
+
+@[simp] theorem sizeOf_def {self : TypeRef} :
+  sizeOf self = self.baseMro.length
+:= rfl
+
+@[simp] theorem length_mro : (mro self).length = self.baseMro.length + 1 := by
+  simp [mro_eq_cons_baseMro]
+
+theorem mem_mro_iff : ty ∈ mro self ↔ ty = self ∨ ty ∈ baseMro self := by
+  simp [mro_eq_cons_baseMro]
+
+@[simp] theorem self_mem_mro : self ∈ mro self := by
+  simp [mro_eq_cons_baseMro]
+
+@[simp] theorem baseMro_subset_mro : baseMro self ⊆ mro self := by
+  simp [mro_eq_cons_baseMro]
+
+private theorem sup_mem_baseMro_sub :
+  sup ∈ baseMro sub → ∀ {ty}, ty ∈ baseMro sup → ty ∈ baseMro sub
+:= by
+  match h_sub:sub.base? with
+  | none =>
+    simp only [baseMro_eq_elim, h_sub, Option.elim_none, List.not_mem_nil]
+    intro sup_eq_sub
+    intro ty
+    simp [sup_eq_sub]
+  | some base =>
+    have sub_baseMro : sub.baseMro = mro base := by
+      simp [h_sub, baseMro_eq_elim]
+    simp only [sub_baseMro, mem_mro_iff]
+    intro h ty
+    intro ty_mem
+    apply Or.inr
+    cases h with
+    | inl sup_eq_sub => simpa [sup_eq_sub] using ty_mem
+    | inr sup_mem_mro_base => exact sup_mem_baseMro_sub sup_mem_mro_base ty_mem
+termination_by sub
+decreasing_by simp [sub_baseMro]
+
+private theorem sup_mem_mro_sub :
+  sup ∈ mro sub → ∀ {ty}, ty ∈ mro sup → ty ∈ mro sub
+:= by
+  simp only [mem_mro_iff]
+  rintro ⟨_ | _⟩ _ ⟨_ | _⟩
+  · simp
+  · simp [*]
+  · simp [*]
+  · apply Or.inr
+    next sup_mem ty ty_mem =>
+    exact sup_mem_baseMro_sub sup_mem ty_mem
+
+def Subtype (self other : TypeRef) : Prop :=
+  other ∈ self.mro
+
+instance : HasSubset TypeRef := ⟨TypeRef.Subtype⟩
+
+theorem Subtype.iff_mem_mro : a ⊆ b ↔ b ∈ mro a := Iff.rfl
+
+def SSubtype (self other : TypeRef) : Prop :=
+  other ∈ self.baseMro
+
+instance : HasSSubset TypeRef := ⟨TypeRef.SSubtype⟩
+
+theorem SSubtype.iff_mem_baseMro : a ⊂ b ↔ b ∈ baseMro a := Iff.rfl
+
+theorem Subtype.iff_eq_or_mem_baseMro : a ⊆ b ↔ (a = b ∨ b ∈ baseMro a) := by
+  grind [Subtype.iff_mem_mro, mem_mro_iff]
+
+theorem Subtype.iff_eq_or_ssubset {a b : TypeRef} : a ⊆ b ↔ (a = b ∨ a ⊂ b) := by
+  rw [Subtype.iff_eq_or_mem_baseMro, SSubtype.iff_mem_baseMro]
+
+@[simp] theorem Subtype.rfl {self : TypeRef} : self ⊆ self := self_mem_mro
+
+@[simp] theorem Subtype.refl (self : TypeRef) : self ⊆ self := self_mem_mro
+
+theorem SSubtype.trans {a b c : TypeRef} : a ⊂ b → b ⊂ c → a ⊂ c := by
+  simp only [SSubtype.iff_mem_baseMro]
+  exact fun h₁ h₂ => sup_mem_baseMro_sub h₁ h₂
+
+instance : Trans (SSubset : TypeRef → TypeRef → Prop) SSubset SSubset :=
+  ⟨SSubtype.trans⟩
+
+theorem Subtype.trans {a b c : TypeRef} : a ⊆ b → b ⊆ c → a ⊆ c  := by
+  simp only [Subtype.iff_mem_mro]
+  exact fun h₁ h₂ => sup_mem_mro_sub h₁ h₂
+
+instance : Trans (Subset : TypeRef → TypeRef → Prop) Subset Subset :=
+  ⟨Subtype.trans⟩
+
+end TypeRef
